progress elpi

code/rocq/elpi.v
@@ -8,61 +8,116 @@ Module Nur (U : Unif).
   Module Run := Run(U).
   Import Run U Language.
 
-  Fixpoint H (ml : list mode) (q : Tm) (h: Tm) s : option Sigma :=
-    match ml,q,h with
-    | [::], Code c, Code c1 => if c == c1 then Some s else None
-    | [:: i & ml], (Comb q a1), (Comb h a2) => obind (H ml q h) (U.matching a1 a2 s) 
-    | [:: o & ml], (Comb q a1), (Comb h a2) => obind (H ml q h) (U.unify a1 a2 s) 
-    | _, _, _ => None
-    end.
-
-  Fixpoint select (query : Tm) (modes:list mode) (rules: list R) sigma : seq (Sigma * R) :=
-    match rules with
-    | [::] => [::]
-    | rule :: rules =>
-      match H modes query rule.(head) sigma with
-      | None => select query modes rules sigma
-      | Some sigma' => (sigma', rule) :: select query modes rules sigma
-      end
-    end.
-
-  Definition F pr query s : seq (Sigma * R) :=
-    let rules := pr.(rules) in
-    let modes := pr.(modes) query in
-    let rules := select query modes rules s in
-    rules.
-
-  Inductive G := g : A -> list (list G) -> G.
+  Inductive G := 
+    | call : Tm -> G
+    | cut : list (list G) -> G.
   Definition alt := (list G).
 
   Definition next_alt {T:Type} a (k : list G -> list alt -> option  T) :=
     if a is [:: gl & a] then k gl a
     else None.
 
-  Definition save_alt a (b: Sigma * R) gs := ([seq g x a | x <- (snd b).(premises)] ++ gs).
+  Definition save_alt_ca (a : A) alts :=
+    match a with
+    | Cut => cut alts
+    | Call t => call t
+    end.
+
+  Definition save_alt a (b: Sigma * R) gs := ([seq save_alt_ca x a | x <- (snd b).(premises)] ++ gs).
   Definition more_alt a bs gs := [seq (save_alt a b1 gs) | b1 <- bs] ++ a.
 
 
   Inductive nur (p: program) : list G ->  list alt -> list alt -> Prop :=
   | StopE a : nur [::] a a
-  | CutE a ca r gl : nur gl ca r -> nur [:: g Cut ca & gl] a r
-  | CallE a ca b bs gl r t s : 
+  | CutE a ca r gl : nur gl ca r -> nur [:: cut ca & gl] a r
+  | CallE a b bs gl r t s : 
     F p t s = [:: b & bs ] -> 
       nur (save_alt a b gl) (more_alt a bs gl) r -> 
-        nur [::g (Call t) ca & gl] a r
+        nur [::call t & gl] a r
   | FailE a g al r : nur a al r -> nur g (a :: al) r.
 
-  Fixpoint state_to_list (A: state) : list alt :=
-    match A with
-    | OK | Top | Bot | KO | Dead => [::]
-    | Goal _ A => [::[::g A [::]]]
-    | Or A _ B => state_to_list A ++ state_to_list B
-    | And A _ B => state_to_list A
+  Definition nur' p a r :=
+    match a with
+    | [::] => False
+    | x :: xs => nur p x xs r
     end.
 
+  Definition add_ca gl (l2 : list alt) : G :=
+    match gl with
+    | call t => call t
+    | cut l1 => cut (l1 ++ l2) end.
+  
+  Definition add_cas lA lB : alt :=
+    [seq add_ca gl lB | gl <- lA].
+
+  Definition add_alt lA lB : list alt :=
+    flatten [seq [seq la ++ lb | lb <- lB] | la <- lA].
+
+  Fixpoint state_to_list (A: state) (bt : list alt) : list alt :=
+    match A with
+    | OK | Top => [::[::]]
+    | Bot | KO | Dead => [::]
+    | Goal _ Cut => [::[::cut [::]]]
+    | Goal _ (Call t) => [::[::call t]]
+    | Or A _ B => 
+      let lB := state_to_list B bt in
+      let lA := state_to_list A (lB ++ bt) in
+      [seq add_cas la bt | la <- lA] ++ lB
+    | And A _ B => 
+      let lA := state_to_list A bt in
+      let lB := state_to_list B bt in
+      add_alt lA lB 
+    end.
+
+  Goal forall p b0 x y z w s1 s2, 
+    state_to_list (
+      And 
+        (Or (Goal p (Call x)) s1 (Goal p (Call y))) b0 
+        (Or (Goal p (Call z)) s2 (Goal p (Call w)))) [::] = 
+      [:: [:: call x; call z];
+      [:: call x; call w];
+      [:: call y; call z];
+      [:: call y; call w]].
+  Proof. by []. Qed.
+
+  Goal forall p a b s1 s2, 
+    state_to_list (
+      Or 
+        (Or (Goal p Cut) s1 (Goal p (Call a))) s2
+        (Goal p (Call b))) [::] = 
+     [:: [:: cut [:: [:: call b]]]; [:: call a]; [:: call b]].
+  Proof. by []. Qed.
+
+  Goal forall b0 p a b c s1 s2, 
+    state_to_list (
+      Or 
+        (Or (And (Goal p (Call c)) b0 (Goal p Cut)) s1 (Goal p (Call a))) s2
+        (Goal p (Call b))) [::] = 
+     [:: [:: call c; cut [:: [:: call b]]]; [:: call a]; [:: call b]].
+  Proof. by []. Qed.
+
+  Definition runElpi A :=
+    forall s p r r1 b,
+      runb s A r b -> nur' p (state_to_list A [::]) r1 -> state_to_list (get_state_run r) [::] = r1.
+  
+  Goal @runElpi OK.
+  Proof.
+    rewrite/runElpi => s p r r1 b/=.
+    inversion 1; subst => //=.
+    - inversion 1; subst.
+      inversion H1; subst => //.
+      case: H8 => _ <-/=.
+
+
+  Lemma runExpandedb {s A s' B x xs}:
+     expandedb s A (Done s' B) b ->
+      state_to_list A [::] = x :: xs ->
+        nur p x xs r1 ->
+          state_to_list (get_state_run (Done s' B)) [::] = r1.
+
   Lemma runElpi {s p A x xs r r1}:
-    state_to_list A = x::xs ->
-    run s A r -> nur p x xs r1 -> state_to_list (get_state_run r) = r1.
+    state_to_list A [::] = x::xs ->
+    run s A r -> nur p x xs r1 -> state_to_list (get_state_run r) [::] = r1.
   Proof.
     move=> + [b H].
     elim: H p x xs r1; clear.
